switched to IfZero; still broken

coq/two/LambdaTwo.v
@@ -68,9 +68,10 @@ Definition eval_kl : nat * nat -> two -> (value -> value -> Prop) ->
                 | TIf t1 t2 t3 =>
                   if Compare_dec.zerop (fst kl) then False
                   else let eval := eval_kl (fst kl - 1, snd kl) _ in
-                       exists b l1,
-                         eval L P pc e t1 (Atom (VBool b) l1) /\
-                         if b then eval L P (l1 ⊔ pc) e t2 a
+                       exists n l1,
+                         eval L P pc e t1 (Atom (VNat n) l1) /\
+                         if Compare_dec.zerop n
+                         then eval L P (l1 ⊔ pc) e t2 a
                          else eval L P (l1 ⊔ pc) e t3 a
               end));
   unfold pair_lt; simpl; omega.
@@ -113,9 +114,10 @@ Lemma eval_kl_eq :
         | TIf t1 t2 t3 =>
           if Compare_dec.zerop (fst kl) then False
           else let eval := eval_kl (fst kl - 1, snd kl) in
-               exists b l1,
-                 eval L P pc e t1 (Atom (VBool b) l1) /\
-                 if b then eval L P (l1 ⊔ pc) e t2 a
+               exists n l1,
+                 eval L P pc e t1 (Atom (VNat n) l1) /\
+                 if Compare_dec.zerop n
+                 then eval L P (l1 ⊔ pc) e t2 a
                  else eval L P (l1 ⊔ pc) e t3 a
       end.
 Proof.
@@ -143,7 +145,7 @@ Proof.
     apply functional_extensionality_ex; intro l1.
     destruct l1; rewrite H'; simpl; try rewrite H'; reflexivity.
   - destruct x1; auto; simpl.
-    apply functional_extensionality_ex; intro b.
+    apply functional_extensionality_ex; intro n.
     apply functional_extensionality_ex; intro l1.
     rewrite H'. reflexivity.
 Qed.
@@ -278,26 +280,26 @@ Qed.
 
 Lemma eval_kl_iftrue :
   forall k l L P pc e t1 t2 t3 l1 a,
-    eval_kl (k, l) L P pc e t1 (Atom (VBool true) l1) ->
+    eval_kl (k, l) L P pc e t1 (Atom (VNat 0) l1) ->
     eval_kl (k, l) L P (l1 ⊔ pc) e t2 a ->
     eval_kl (S k, l) L P pc e (TIf t1 t2 t3) a.
 Proof.
   introv Ht1 Ht2.
   rewrite eval_kl_eq. simpl.
   replace (k - 0) with k by omega.
-  exists true l1. auto.
+  exists 0 l1. auto.
 Qed.
 
 Lemma eval_kl_iffalse :
-  forall k l L P pc e t1 t2 t3 l1 a,
-    eval_kl (k, l) L P pc e t1 (Atom (VBool false) l1) ->
+  forall k l L P pc e t1 t2 t3 l1 n a,
+    eval_kl (k, l) L P pc e t1 (Atom (VNat (S n)) l1) ->
     eval_kl (k, l) L P (l1 ⊔ pc) e t3 a ->
     eval_kl (S k, l) L P pc e (TIf t1 t2 t3) a.
 Proof.
   introv Ht1 Ht3.
   rewrite eval_kl_eq. simpl.
   replace (k - 0) with k by omega.
-  exists false l1. auto.
+  exists (S n) l1. auto.
 Qed.
 
 Lemma eval_kl_if_inv :
@@ -305,22 +307,22 @@ Lemma eval_kl_if_inv :
     eval_kl (k, l) L P pc e (TIf t1 t2 t3) a ->
     (exists k' l1,
        k = S k' /\
-       eval_kl (k', l) L P pc e t1 (Atom (VBool true) l1) /\
+       eval_kl (k', l) L P pc e t1 (Atom (VNat 0) l1) /\
        eval_kl (k', l) L P (l1 ⊔ pc) e t2 a) \/
-    (exists k' l1,
+    (exists k' n l1,
        k = S k' /\
-       eval_kl (k', l) L P pc e t1 (Atom (VBool false) l1) /\
+       eval_kl (k', l) L P pc e t1 (Atom (VNat (S n)) l1) /\
        eval_kl (k', l) L P (l1 ⊔ pc) e t3 a).
 Proof.
   intros.
   rewrite eval_kl_eq in H.
   destruct k; simpl in H.
   - inversion H.
-  - destruct H as [b [l1 [H1 H2]]].
+  - destruct H as [n [l1 [H1 H2]]].
     replace (k - 0) with k in * by omega.
-    destruct b.
+    destruct n.
     + left. exists k l1. auto.
-    + right. exists k l1. auto.
+    + right. exists k n l1. auto.
 Qed.
 
 Definition eval (L : two) (P : value -> value -> Prop)
